Progress towards reifying functions

coq/theories/automation/Automation.v
@@ -1,11 +1,13 @@
 From impboot Require Import utils.Core.
 From coqutil Require Import dlet.
 Require Import impboot.functional.FunValues.
-Require Import impboot.functional.FunSyntax.
+(* Require Import impboot.functional.FunSyntax. *)
 Require Import impboot.functional.FunSemantics.
 Require Import impboot.automation.AutomationLemmas.
 Require Import impboot.utils.Llist.
 From Ltac2 Require Import Ltac2 Std List Constr RedFlags Message.
+Import Ltac2.Constr.Unsafe.
+From coqutil Require Import Tactics.reference_to_string.
 Require Import Coq.derive.Derive.
 
 Ltac rewrite_let := match goal with
@@ -84,8 +86,11 @@ Qed. *)
       ([encode (letd x := 1 in x + n - m)], empty_state))
   As f1_rpoof. *)
 
+(* HOL4-ish approach *)
+
 (* TODO(kπ) track free variables to name let_n (use Ltac2.Free) *)
 Ltac2 rec compile (e : constr) (cenv : constr list) : constr :=
+  print (of_constr e);
   lazy_match! e with
   | (dlet ?val ?body) =>
     let compiled_val := compile val cenv in
@@ -101,6 +106,7 @@ Ltac2 rec compile (e : constr) (cenv : constr list) : constr :=
     (* eval v1 *) $compiled_val
     (* eval f *) $compiled_body
     )
+  (* bool *)
   | true =>
     open_constr:(auto_bool_T
     (* env *) _
@@ -155,6 +161,7 @@ Ltac2 rec compile (e : constr) (cenv : constr list) : constr :=
     (* eval x_t *) $compile_t
     (* eval x_f *) $compile_f
     )
+  (* num *)
   | (?n1 + ?n2) =>
     let compile_n1 := compile n1 cenv in
     let compile_n2 := compile n2 cenv in
@@ -220,8 +227,41 @@ Ltac2 rec compile (e : constr) (cenv : constr list) : constr :=
     (* eval y *) $compile_t
     (* eval z *) $compile_f
     )
-
-    | ?x =>
+  (* list *)
+  | [] =>
+    open_constr:(auto_list_nil
+    (* env *) _
+    (* s *) _
+    )
+  | (?x :: ?xs) =>
+    let compile_x := compile x cenv in
+    let compile_xs := compile xs cenv in
+    open_constr:(auto_list_cons
+    (* env *) _
+    (* s *) _
+    (* x1 x2 *) _ _
+    (* x *) $x
+    (* xs *) $xs
+    (* eval x1 *) $compile_x
+    (* eval x2 *) $compile_xs
+    )
+  | (list_CASE ?v0 ?v1 ?v2) =>
+    let compile_v0 := compile v0 cenv in
+    let compile_v1 := compile v1 cenv in
+    let compile_v2 := (fun (xh : constr) (xt : constr) => compile (eval_cbv beta open_constr:($v2 $xh $xt)) (xh :: xt :: cenv)) in
+    open_constr:(auto_list_case
+    (* env *) _
+    (* s *) _
+    (* x0 x1 x2 *) _ _ _
+    (* n1 n2 *) _ _
+    (* v0 v1 v2 *) $v0 $v1 $v2
+    (* eval x0 *) $compile_v0
+    (* eval x1 *) $compile_v1
+    (* TODO(kπ) not sure if the &-references are correct *)
+    (* eval x2 *) (fun xh xt _ => ltac2:(Control.refine (fun () => (compile_v2 &xh &xt))))
+    (* NoDup *) _
+    )
+  | ?x =>
     (* TODO(kπ) We should handle shadowing things (or avoid any type of shadowing in the implementation) *)
     match find_opt (equal x) cenv with
     | Some _ =>
@@ -241,22 +281,150 @@ Ltac2 rec compile (e : constr) (cenv : constr list) : constr :=
     end
   end.
 
+Ltac2 rec constr_to_list (c : constr) : constr list :=
+  match! c with
+  | [] => []
+  | ?x :: ?xs => x :: constr_to_list xs
+  end.
+
+(* TODO(kπ) this only works when fun is the top level App in the compiled
+expression, otherwise we might have to have a funtion from a constr (that is a
+string) to reference. So constr stirng to string? *)
+Ltac2 rec fun_ident (c : constr) : reference :=
+  match kind c with
+  | App f _ => reference_of_constr f
+  | _ => reference_of_constr c
+  end.
+
 Ltac2 doauto () :=
   match! goal with
   | [ |- _ |-- (_, _) ---> ([encode ?g], _) ] =>
     refine (compile g []);
     intros;
     eauto with fenvDb
+  (* TODO(kπ) we need to know whether it is the currently compiled function at some point  *)
+  | [ h : (lookup_fun ?fname _ = _) |- eval_app ?fname ?args _ (encode ?g, _) ] =>
+    let argsl := constr_to_list args in
+    let f_ident := fun_ident g in
+    let g_norm := eval_unfold [(f_ident, AllOccurrences)] g in
+    print (of_string "g_norm");
+    print (of_constr g_norm);
+    let compile_g := compile g_norm argsl in
+    let h_ref := Control.hyp h in
+    refine open_constr:(trans_app
+    (* n *) _
+    (* params *) _
+    (* vs *) $args
+    (* body *) _
+    (* s *) _
+    (* s1 *) _
+    (* v *) _
+    (* eval body *) $compile_g
+    (* params length eq *) _
+    (* lookup_fun *) $h_ref
+    )
   end.
 
 Lemma arith_example : forall n,
   exists prog,
     FEnv.empty |-- (prog, empty_state) --->
-    ([encode (letd x := 1 in x + n)], empty_state).
+    ([encode
+      (letd x := 1 in x + n)
+    ], empty_state).
 Proof.
   intros; eexists.
   doauto ().
   Show Proof.
+  exact "a"%string.
+Qed.
+
+Lemma list_example : forall (n : nat),
+  exists prog,
+    FEnv.empty |-- (prog, empty_state) --->
+    ([encode
+      (letd l := [1; 2; 3] in
+      letd fnil := n in
+      list_CASE l fnil (fun (x : nat) _ => x + 1))
+    ], empty_state).
+Proof.
+  intros; eexists.
+  (* Set Ltac2 Backtrace. *)
+  doauto ().
+  Show Proof.
+  (* TODO(kπ) Common crush tactic for these vvv (free_vars, NoDup, in_nil) *)
+  all: unfold FunProperties.free_vars; simpl.
+  all: try (eapply NoDup_cons); try (eapply in_nil); try (eapply NoDup_nil).
+  (* TODO(kπ) Also a common crush tactic for picking variable names *)
+  (* TODO(kπ): Slow vvv *)
+  (* - exact ("a"%string).
+  - exact ("b"%string).
+  - exact ("a"%string).
+  - inversion e; subst; rewrite FEnv.lookup_insert_neq; try (rewrite FEnv.lookup_insert_eq); auto.
+    unfold name_enc, name_enc_l; simpl; ltac1:(lia).
+  - exact ("c"%string).
+  - exact ("d"%string). *)
+Admitted.
+
+Lemma list_example2 : forall (n : nat),
+  exists prog,
+    FEnv.empty |-- (prog, empty_state) --->
+    ([encode
+      (letd l := [1; 2; 3] in
+      letd fnil := n in
+      list_CASE l fnil (fun (x : nat) xs =>
+        list_CASE xs (x + 99) (fun (y : nat) _ => y + 1)
+      ))
+    ], empty_state).
+Proof.
+  intros; eexists.
+  (* Set Ltac2 Backtrace. *)
+  doauto ().
+  Show Proof.
+  (* TODO(kπ) Common crush tactic for these vvv (free_vars, NoDup, in_nil) *)
+  all: unfold FunProperties.free_vars; simpl.
+  all: try (eapply NoDup_cons); try (eapply in_nil); try (eapply NoDup_nil).
+  (* TODO(kπ) Also a common crush tactic for picking variable names *)
+  (* TODO(kπ): Slow vvv *)
+  (* - exact ("a"%string).
+  - exact ("b"%string).
+  - exact ("c"%string).
+  - exact ("b"%string).
+  - exact ("a"%string).
+  - exact ("f"%string).
+  - eapply not_in_cons; split; try (eapply in_nil); unfold name_enc, name_enc_l; simpl; ltac1:(lia).
+  - eapply NoDup_cons; try (eapply in_nil); try (eapply NoDup_nil).
+  - inversion e; subst; rewrite FEnv.lookup_insert_neq; try (rewrite FEnv.lookup_insert_eq); auto.
+    unfold name_enc, name_enc_l; simpl; ltac1:(lia).
+  - inversion e; subst; rewrite FEnv.lookup_insert_neq; try (rewrite FEnv.lookup_insert_eq); auto.
+    unfold name_enc, name_enc_l; simpl; ltac1:(lia).
+  - exact ("g"%string).
+  - exact ("h"%string). *)
+Admitted.
+
+Definition foo (n : nat) : nat :=
+  letd x := 1 in
+  letd y := n + x in
+  y.
+
+Lemma function_example : forall (s : state) (n : nat),
+  exists prog,
+    lookup_fun (name_enc "foo") s.(funs) = Some ([name_enc "n"], prog) ->
+      eval_app (name_enc "foo") [encode n] s (encode (foo n), s).
+Proof.
+  intros; eexists; intros.
+
+  (* TODO(kπ) This inlined the `y` :thinking: *)
+  doauto ().
+  Show Proof.
+  - simpl; ltac1:(reflexivity).
+  - exact "a"%string.
+  - exact "b"%string.
+  - exact "a"%string.
+  - exact "b"%string.
+  Unshelve.
+Admitted.
+
+(*
   all: simpl.
   all: try (eapply auto_num_const).
   all: try (doauto ()).
@@ -282,4 +450,5 @@ Proof.
   repeat (autostep; intros).
   Show Proof.
 
-  (* eauto with automation. *)
+  eauto with automation. *)
+
